Inspiration

code/ecdsap256/Hacl.Impl.Q.LowLevel.fst
@@ -21,6 +21,8 @@ open Lib.Loops
 
 open Lib.IntTypes.Intrinsics
 
+open Hacl.Impl.Q.RandomFor
+
 
 #set-options "--fuel 0 --ifuel 0 --z3rlimit 200"
 
@@ -55,12 +57,16 @@ val generateRandomShares:
   x: felem 
   -> shares: size_t 
   -> l: lbuffer uint64 (size 4 *. shares) 
+  -> lenRandomness: size_t
+  -> randomness: lbuffer uint8 lenRandomness
+  
   -> Stack unit 
     (requires fun h -> True)
     (ensures fun h0 _ h1 -> True)
 
 
-let generateRandomShares x shares l = 
+let generateRandomShares x shares l lenRandomness randomness = 
+  let h = ST.get() in 
   let last = sub l (size 4 *. (shares -. 1ul)) (size 4) in 
   let inv h (i: nat) = True in 
   for 0ul (shares -. 1ul) inv (fun i -> 
@@ -102,22 +108,18 @@ val add4_secr: x: felem
 
 
 let add4_secr x y result n randomness = 
-  push_frame();
-    let shares = create (size 4 *. n) (u64 0) in
-    copy shares randomness;
-    generateRandomShares x n shares;
-    let inv h (i: nat) = True in 
-    
+  let shares = create (size 4 *. n) (u64 0) in
+  copy shares randomness;
+  generateRandomShares x n shares n randomness;
+  
+  let shares2 = create (size 4 *. n) (u64 0) in 
+  copy shares randomness;
+  generateRandomShares y n shares2 n randomness;
 
-    let shares2 = create (size 4 *. n) (u64 0) in 
-    copy shares randomness;
-    generateRandomShares y n shares2;
-    
-  for 0ul n inv (fun i -> 
-    let share = sub shares (size 4 *. i) (size 4) in  
-    let share2 = sub shares2 (size 4 *. i) (size 4) in 
-    p256_add share share2 share);
+  let inv = fun h -> True in 
 
+  forRandom n shares shares2 shares inv p256_add n randomness;
+  
   rejoinShares n shares result;
   
 
